Verified unbalanced and red black sets

examples/miniML/okasaki-examples/RedBlackSetScript.sml
@@ -1,5 +1,5 @@
 open bossLib Theory Parse boolTheory pairTheory Defn Tactic boolLib 
-open relationTheory miscTheory pred_setTheory lcsymtacs;
+open relationTheory miscTheory pred_setTheory pred_setSimps lcsymtacs;
 
 val fs = full_simp_tac (srw_ss ())
 val rw = srw_tac []
@@ -17,6 +17,22 @@ color = Red | Black`;
 val _ = Hol_datatype `
 tree = Empty | Node of color => tree => 'a => tree`;
 
+val tree_distinct = fetch "-" "tree_distinct"
+val tree_nchotomy = fetch "-" "tree_nchotomy"
+
+val redblack_set_to_set_def = Define `
+(redblack_set_to_set Empty = {}) ∧
+(redblack_set_to_set (Node _ t1 x t2)  =
+  {x} ∪ redblack_set_to_set t1 ∪ redblack_set_to_set t2)`;
+
+val redblack_set_ok_def = Define `
+(redblack_set_ok lt Empty = T) ∧
+(redblack_set_ok lt (Node _ t1 x t2) = 
+  redblack_set_ok lt t1 ∧
+  redblack_set_ok lt t2 ∧
+  (!y. y ∈ redblack_set_to_set t1 ⇒ lt y x) ∧
+  (!y. y ∈ redblack_set_to_set t2 ⇒ lt x y))`;
+
 val empty_def = Define `
 empty = Empty`;
 
@@ -29,6 +45,18 @@ val member_def = Define `
     member lt x b
   else
     T)`;
+
+val member_thm = Q.store_thm ("member_thm",
+`!lt t x. 
+  StrongLinearOrder lt ∧
+  redblack_set_ok lt t 
+  ⇒ 
+  (member lt x t = x ∈ redblack_set_to_set t)`,
+induct_on `t` >>
+rw [member_def, redblack_set_ok_def, redblack_set_to_set_def] >>
+fs [StrongLinearOrder, StrongOrder, irreflexive_def, transitive_def,
+    trichotomous] >>
+metis_tac []);
 
 val balance_def = Define `
 (balance Black (Node Red (Node Red a x b) y c) z d =
@@ -45,6 +73,29 @@ val balance_def = Define `
 
 (balance col a x b = Node col a x b)`;
 
+val balance_ind = fetch "-" "balance_ind";
+
+val balance_node = Q.prove (
+`!c t1 x t2. ∃c' t1' x' t2'. (balance c t1 x t2 = Node c' t1' x' t2')`,
+recInduct balance_ind >>
+srw_tac [PRED_SET_AC_ss] [balance_def]);
+
+val balance_set = Q.prove (
+`!c t1 x t2.
+  redblack_set_to_set (balance c t1 x t2) = 
+  redblack_set_to_set (Node c t1 x t2)`,
+recInduct balance_ind >>
+srw_tac [PRED_SET_AC_ss] [balance_def, redblack_set_to_set_def]);
+
+val balance_ok = Q.prove (
+`!c t1 x t2.
+  transitive lt ∧
+  redblack_set_ok lt (Node c t1 x t2) ⇒
+  redblack_set_ok lt (balance c t1 x t2)`,
+recInduct balance_ind >>
+rw [transitive_def, balance_def, redblack_set_ok_def, redblack_set_to_set_def] >>
+metis_tac []);
+
 val ins_def = Define `
 (ins lt x Empty = Node Red Empty x Empty) ∧
 (ins lt x (Node col a y b) =
@@ -55,9 +106,66 @@ val ins_def = Define `
   else
     Node col a y b)`;
 
+val ins_node = Q.prove (
+`!lt x t. ?c t1 y t2. (ins lt x t = Node c t1 y t2)`,
+cases_on `t` >>
+rw [ins_def] >>
+metis_tac [balance_node]);
+
+val ins_set = Q.prove (
+`∀lt x t.
+  StrongLinearOrder lt ⇒
+  (redblack_set_to_set (ins lt x t) = {x} ∪ redblack_set_to_set t)`,
+induct_on `t` >>
+rw [redblack_set_to_set_def, ins_def, balance_set] >>
+fs [] >>
+srw_tac [PRED_SET_AC_ss] [] >>
+`x = a` by (fs [StrongLinearOrder, StrongOrder, irreflexive_def, 
+                transitive_def, trichotomous] >>
+            metis_tac []) >>
+rw []);
+
+val ins_ok = Q.prove (
+`!lt x t.
+  StrongLinearOrder lt ∧
+  redblack_set_ok lt t 
+  ⇒ 
+  redblack_set_ok lt (ins lt x t)`,
+induct_on `t` >>
+rw [redblack_set_ok_def, ins_def, redblack_set_to_set_def] >>
+match_mp_tac balance_ok >>
+rw [redblack_set_ok_def] >>
+imp_res_tac ins_set >>
+fs [StrongLinearOrder, StrongOrder]);
+
 val insert_def = Define `
 insert lt x s =
   case ins lt x s of
      | Node _ a y b => Node Black a y b`;
+
+val insert_set = Q.store_thm ("insert_set",
+`∀lt x t.
+  StrongLinearOrder lt ⇒
+  (redblack_set_to_set (insert lt x t) = {x} ∪ redblack_set_to_set t)`,
+rw [insert_def] >>
+`?c t1 y t2. ins lt x t = Node c t1 y t2` by metis_tac [ins_node] >>
+rw [redblack_set_to_set_def] >>
+`redblack_set_to_set (ins lt x t) = redblack_set_to_set (Node c t1 y t2)` 
+         by metis_tac [] >>
+fs [] >>
+imp_res_tac ins_set >>
+fs [redblack_set_to_set_def]);
+
+val insert_ok = Q.store_thm ("insert_ok",
+`!lt x t.
+  StrongLinearOrder lt ∧
+  redblack_set_ok lt t 
+  ⇒ 
+  redblack_set_ok lt (insert lt x t)`,
+rw [insert_def] >>
+`?c t1 y t2. ins lt x t = Node c t1 y t2` by metis_tac [ins_node] >>
+rw [] >>
+`redblack_set_ok lt (Node c t1 y t2)` by metis_tac [ins_ok] >>
+fs [redblack_set_ok_def]);
 
 val _ = export_theory ();
