examples/miniML/okasaki-examples/UnbalancedSetScript.sml
@@ -1,5 +1,5 @@
 open bossLib Theory Parse boolTheory pairTheory Defn Tactic boolLib 
-open relationTheory miscTheory pred_setTheory lcsymtacs;
+open relationTheory miscTheory pred_setTheory pred_setSimps lcsymtacs;
 
 val fs = full_simp_tac (srw_ss ())
 val rw = srw_tac []
@@ -14,6 +14,19 @@ val _ = new_theory "UnbalancedSet"
 val _ = Hol_datatype `
 tree = Empty | Node of tree => 'a => tree`;
 
+val unbalanced_set_to_set_def = Define `
+(unbalanced_set_to_set Empty = {}) ∧
+(unbalanced_set_to_set (Node t1 x t2)  =
+  {x} ∪ unbalanced_set_to_set t1 ∪ unbalanced_set_to_set t2)`;
+
+val unbalanced_set_ok_def = Define `
+(unbalanced_set_ok lt Empty = T) ∧
+(unbalanced_set_ok lt (Node t1 x t2) = 
+  unbalanced_set_ok lt t1 ∧
+  unbalanced_set_ok lt t2 ∧
+  (!y. y ∈ unbalanced_set_to_set t1 ⇒ lt y x) ∧
+  (!y. y ∈ unbalanced_set_to_set t2 ⇒ lt x y))`;
+
 val empty_def = Define `
 empty = Empty`;
 
@@ -27,6 +40,18 @@ val member_def = Define `
   else
     T)`;
 
+val member_thm = Q.store_thm ("member_thm",
+`!lt t x. 
+  StrongLinearOrder lt ∧
+  unbalanced_set_ok lt t 
+  ⇒ 
+  (member lt x t = x ∈ unbalanced_set_to_set t)`,
+induct_on `t` >>
+rw [member_def, unbalanced_set_ok_def, unbalanced_set_to_set_def] >>
+fs [StrongLinearOrder, StrongOrder, irreflexive_def, transitive_def,
+    trichotomous] >>
+metis_tac []);
+
 val insert_def = Define `
 (insert lt x Empty = Node Empty x Empty) ∧
 (insert lt x (Node a y b) =
@@ -36,5 +61,26 @@ val insert_def = Define `
     Node a y (insert lt x b)
   else
     Node a y b)`;
+
+val insert_set = Q.store_thm ("insert_set",
+`∀lt x t.
+  StrongLinearOrder lt ⇒
+  (unbalanced_set_to_set (insert lt x t) = {x} ∪ unbalanced_set_to_set t)`,
+induct_on `t` >>
+srw_tac [PRED_SET_AC_ss] [insert_def, unbalanced_set_to_set_def] >>
+`x = a` by (fs [StrongLinearOrder, StrongOrder, irreflexive_def, 
+                transitive_def, trichotomous] >>
+            metis_tac []) >>
+rw []);
+
+val insert_ok = Q.store_thm ("insert_ok",
+`!lt x t.
+  StrongLinearOrder lt ∧
+  unbalanced_set_ok lt t 
+  ⇒ 
+  unbalanced_set_ok lt (insert lt x t)`,
+induct_on `t` >>
+rw [unbalanced_set_ok_def, insert_def, unbalanced_set_to_set_def, insert_set] >>
+metis_tac []);
 
 val _ = export_theory ();
